---
title: Abstract Algebra by Pinter, Chapter 18
author: Amir Taaki
header-includes: |
    - \usepackage{mathrsfs}
    - \usepackage{mathtools}
    - \usepackage{extpfeil}
    - \DeclareMathOperator\cis{cis}
    - \DeclareMathOperator\ker{ker}
    - \DeclareMathOperator\ord{ord}
    - \DeclareMathOperator\gcd{gcd}
    - \DeclareMathOperator\lcm{lcm}
    - \DeclareMathOperator\rad{rad}
    - \DeclareMathOperator\mod{mod}
abstract: Chapter 18 on Ideals
---

# A. Examples of Subrings

## Q1

$$\{ x + \sqrt{3}y : x, y \in \mathbb{Z} \}$$

Closed wrt subtraction

$$(x + \sqrt{3}y)(v + \sqrt{3}w) = xv + \sqrt{3}(yv + xw) + 3yw \in \mathbb{R}$$

Thus it's a subring.

## Q2

As before, it's closed under subtraction and multiplication.

## Q3

$$\{x2^y : x, y \in \mathbb{Z}\}$$

Closed under multiplication because:

$$x_1 2^{y_1} \cdot x_2 2^{y_2} = (x_1 x_2) 2^{y_1 + y_2}$$

Also contains negatives since $x \in \mathbb{Z}$.

To show closure under addition is trivial for positive powers since

$$x 2^y + v 2^w = x 2^{(y - w)} 2^w + v 2^w = (x 2^{(y - w)} + v) 2^w$$

Now for the negative case, assume $y > w$, hence $y - w$ is positive and the formulation still holds.

## Q4

The sum and product of continuous functions are continuous.

## Q5

The sum and product on any interval $[0, 1]$ also remains continuous, and hence also includes $\mathcal{C}$

## Q6

Addition and negatives remain in $\mathcal{M}_2(\mathbb{R})$ as does multiplication
$$
\begin{pmatrix}
0 & 0\\
0 & x
\end{pmatrix}
\begin{pmatrix}
0 & 0\\
0 & y
\end{pmatrix}
=
\begin{pmatrix}
0 & 0\\
0 & xy
\end{pmatrix}
$$

# B. Examples of Ideals

## Q1

*Identify which of the following are ideals of $\mathbb{Z} \times \mathbb{Z}$*

### $\{(n, n) : n \in \mathbb{Z}\}$

\begin{align*}
(n, n) + (m, m) &= (m + n, m + n) \in I \\
-(n, n) &= (-n, -n) \in I \\
(n, n) \cdot (a, b) &= (na, nb) \notin I
\end{align*}

Not an ideal.

### $\{(5n, 0) : n \in \mathbb{Z}\}$

\begin{align*}
(5m, 0) + (5n, 0) &= (5(m + n), 0) \in I \\
-(5n, 0) &= (5(-n), 0) \in I \\
(5n, 0) \cdot (a, b) = (5(na), 0) \in I
\end{align*}

Is an ideal.

### $\{(n, m) : n + m \text{ is even }\}$

\begin{align*}
(n_1, m_1) + (n_2, m_2) &= (n_1 + n_2, m_1 + m_2) \in I \\
-(n, m) \in I \\
(n, m) \cdot (a, b) &= (na, mb)
\end{align*}

$na$ is even and $mb$ is even, so $na + mb$ is even so $(na, mb) \in I$.

Is an ideal.

### $\{(2n, 3m) : n, m \in \mathbb{Z}\}$

\begin{align*}
(2n_1, 3m_1) + (2n_2, 3m_2) &= (2(n_1 + n_2), 3(m_1 + m_2)) \in I \\
-(2n, 3m) &= (2(-n), 3(-m)) \in I \\
(2n, 3m) \cdot (a, b) &= (2na, 3mb) \in I
\end{align*}

Is an ideal

## Q2

*List all the ideals of $\mathbb{Z}_{12}$*

$\mathbb{Z}_{12} = \langle 1 \rangle$ and is cyclic. All subgroups are also cyclic.

* $\mathbb{Z}_{12} = <1> = <5> = <7> = <11>$ because $\gcd(m, 12) = 1$
* $<4> = <8>, <4> = \{4, 8, 0\}$
* $<3> = <9>, <3> = \{3, 6, 9, 0\}$
* $<2> = <10>, <2> = \{2, 4, 6, 8, 10, 0\}$
* $<6> = \{6, 0\}$
* $<0> = \{0\}$

Let $m \in \bar{m} = <m>$, then $<m> = \{mj : j \in \mathbb{Z}_{12}\}$

Let $x \in <m>$ and $y \in \mathbb{Z}_{12}$, since $x \in <m>$, then $x = mj$ for some $j \in \mathbb{Z}_{12}$, thus $xy = mjy$, thus $<m>$ is an ideal of $\mathbb{Z}_{12}$.

Ideals are $<0>, <1>, <2>, <3>, <4>, <6>$

## Q3

See previous exercise

## Q4

$$
\begin{pmatrix}
1 & 1\\
1 & 1
\end{pmatrix}
\begin{pmatrix}
0 & 0\\
0 & x
\end{pmatrix}
=
\begin{pmatrix}
0 & x\\
0 & x 
\end{pmatrix}
\notin \mathcal{M}_2(\mathbb{R})
$$

## Q5

The product of a continuous and non-continuous function are non-continuous, hence $\mathcal{C}(\mathbb{R})$ is not an ideal of $\mathcal{F}(\mathbb{R})$

## Q6

### a

Assume he means multiplication here.
$$f(x) \cdot g(x) = 0 \quad \forall x \in \mathbb{Q}$$
Thus $f \cdot g \in I$

### b

Likewise $f(0) g(0) = 0 g(0) = 0$, so $f \cdot g \in I$

## Q7

Ideals of $P_3$ such that $AB = A \cap B \in I$. See also 17D5

$$P_3 = \{ \varnothing, \{a\}, \{b\}, \{c\}, \{a, b\}, \{a, c\}, \{b, c\}, \{a, b, c\}\}$$

Any subgroup must contain $\varnothing$.

$A + A = \varnothing$ so $A$ is its own negative.

$\{\varnothing, \{a\}\}$, $\{\varnothing, \{b\}\}$, $\{\varnothing, \{c\}\}$ are all ideals since $\{a\}\{a, c\} = \{a\}$ and $\{a\}\{b, c\} = \varnothing$.

Likewise $\{\varnothing, \{a\}, \{c\}, \{a, c\}\}$, $\{\varnothing, \{a\}, \{b\}, \{a, b\}\}$, $\{\varnothing, \{b\}, \{c\}, \{b, c\}\}$ since $\{a, c\} \{b, c\} = \{c\}$

Lastly we have $P_3$ itself

## Q8

Example of a non-ideal subring is $\{\varnothing, \{a, c\}\}$ which is closed under addition, negatives and multiplication.

## Q9

$$A = \langle (1, 1) \rangle = \{(0, 0), (1,1), (2,2) \}$$

# C. Elementary Properties of Subrings

## Q1

Let $x \in B$ and since $B$ is a ring then $0 \in B$, thus $0 - x = -x \in B$.

So $B$ is closed wrt negatives and hence addition since $x - (-y) = x + y \in B$

## Q2

As per part 1

## Q3

A ring is a group under addition. Hence order of a subring divides ring by Lagrange.

## Q4

$A$ has no zero divisors, hence neither does $B$ $\implies$ $B$ is an integral domain.

## Q5

$B$ is a subring of field $F$. Let $b \in B, b \neq 0$, then $b^{-1} \in F$ (because $F$ is a field and contains inverses). Every field is an integral domain, hence so is $B$.

## Q6

$F$ is a commutative ring with inverses and unity.

Since $B$ is a subring, it also is commutative.

Since $B$ also contains inverses and is closed wrt multiplication, it must contain $1_F$.

Thus $B$ is a field.

## Q7

### a

$$B = \langle 2 \rangle = \{ 0, 2, 4, \dots, 16 \}$$

### b

$$B = \langle 9 \rangle = \{ 0, 9 \}$$

## Q8

$$f(e) = e$$
$$f(x_1 + x_2) = f(x_1) + f(x_2)$$
$$f(x_1 x_2) = f(x_1) f(x_2)$$

But $\forall x \in B \quad f(x) = x$
$$x_1, x_2 \in B$$
$$ x_1 + x_2 = f(x_1) + f(x_2) = f(x_1 + x_2)$$
Likewise for multiplication.

Since $A$ is a ring $\forall -x \in A$ st $x + (-x) = e$ but $x \in B$

$$f(x) + f(-x) = f(e) = f(x + (-x)) = x + (-x)$$
Hence $-x \in B$ also.

## Q9

$$ax = xa \qquad bx = xb$$
$$(a + b)x = x(a + b)$$
So $a + b$ also is in the center.
$$(ab)x = axb = x(ab)$$
Finally $0x = 0 = x0$
$$-a \in A$$
$$-ax = -(ax) = -(xa) = -xa$$
By associativity.

# D. Elementary Properties of Ideals

## Q1

*Explain why $J$ is an ideal of $A$ iff $J$ is closed with respect to subtraction and $J$ absorbs products in $A$.*

$$0 - x = -x \in J$$
$$x - (-y) = x + y \in J$$

So $J$ is closed wrt negatives and addition from the statement about subtraction.

## Q2

*If $A$ is a ring with unity, prove that $J$ is an ideal of $A$ iff $J$ is closed with respect to addition and $J$ absorbs products in $A$.*

Note that $A$ is a ring with unity, and by definition must include $-1$.

Then note that since $J$ absorbs products, that $(-1)\cdot a = -a \in J$.

## Q3

*Prove that the intersection of any two ideals of $A$ is an ideal of $A$.*

1. Since $x, y \in I_j$, and $I_j$ is an ideal, $x - y \in I_j, \forall j \in J$. Therefore $x - y \in \bigcap_{j \in J} I_j = I$.
2. Since $x \in I_j, rx \in I_j, \forall j \in J$. Therefore $rx \in I$.

## Q4

*Prove that $J$ is an ideal of $A$ and $1 \in J$, then $J = A$.*

Since ideals absorb products, then if $1 \in J$, then since $a \cdot 1 = a \in J$, then $J = A$.

## Q5

*Prove that if $J$ is an ideal of $A$ and $J$ contains an invertible element $a$ of $A$, then $J = A$.*

$$a \cdot a^{-1} = 1 \in J$$
By previous exercise $J = A$.

## Q6

*Explain why a field $F$ can have no nontrivial ideals.*

Every nonzero element of a field is invertible. Hence the only ideals are $\{0\}$ or $F$ itself.

# E. Examples of Homomorphisms

## Q1

Let $f, g \in \mathcal{F}(\mathbb{R})$

$$\phi(f + g) = (f + g)(0) = f(0) + g(0) = \phi(f) + \phi(g)$$
$$\phi(f \cdot g) = (f \cdot g)(0) = f(0)g(0) = \phi(f)\phi(g)$$

$$K = \{f \in \mathcal{F}(\mathbb{R}) : f(0) = 0 \}$$
Range is $[-\infty, \infty]$.

## Q2

$$h: \mathbb{R} \times \mathbb{R} \rightarrow \mathbb{R}$$
$$h(x, y) = x$$
$$h(x_1 + x_2, y_1 + y_2) = x_1 + x_2 = h(x_1, y_1) + h(x_2, y_2)$$
$$h(x_1 x_2, y_1 y_2) = x_1 x_2 = h(x_1, y_1) h(x_2 y_2)$$
\begin{align*}
K &= \{ x, y \in \mathbb{R} \times \mathbb{R} : h(x, y) = 0 \} \\
  &= \{ (0, y) : y \in \mathbb{R} \}
\end{align*}
Range is $[-\infty, \infty]$

## Q3

$$h : \mathbb{R} \rightarrow \mathcal{M}_2(\mathbb{R})$$
$$h(x) =
\begin{pmatrix}
x & 0\\
0 & 0
\end{pmatrix}
$$
$$h(x + y)
=
\begin{pmatrix}
x + y & 0\\
0 & 0
\end{pmatrix}
=
\begin{pmatrix}
x & 0\\
0 & 0
\end{pmatrix}
+
\begin{pmatrix}
y & 0\\
0 & 0
\end{pmatrix}
= h(x) + h(y)$$
$$h(x y)
=
\begin{pmatrix}
x y & 0\\
0 & 0
\end{pmatrix}
=
\begin{pmatrix}
x & 0\\
0 & 0
\end{pmatrix}
\begin{pmatrix}
y & 0\\
0 & 0
\end{pmatrix}
= h(x) h(y)$$
$$K = \{ 0 \}$$
Range is 
$$
\begin{pmatrix}
\pm \infty & 0\\
0 & 0
\end{pmatrix}
$$

## Q4

$$h: \mathbb{R} \times \mathbb{R} \rightarrow \mathcal{M}_2(\mathbb{R})$$
$$h(x, y) =
\begin{pmatrix}
x & 0\\
0 & y
\end{pmatrix}
$$
\begin{align*}
h(x_1 + x_2, y_1 + y_2) &=
\begin{pmatrix}
x_1 + x_2 & 0\\
0 & y_2 + y_2
\end{pmatrix} \\
&=
\begin{pmatrix}
x_1 & 0\\
0 & y_1
\end{pmatrix}
+
\begin{pmatrix}
x_2 & 0\\
0 & y_2
\end{pmatrix}
\\
&= h(x_1, y_1) + h(x_2, y_2)
\end{align*}
$$K = \{(0, 0) \}$$
Range is
$$
\begin{pmatrix}
\pm \infty & 0\\
0 & \pm \infty
\end{pmatrix}
$$

## Q5

$$f: \mathbb{R} \times \mathbb{R} \rightarrow \mathcal{M}_2(\mathbb{R})$$
$$f(x, y) =
\begin{pmatrix}
x & 0\\
y & 0
\end{pmatrix}
$$

\begin{align*}
f(x_1 + x_2, y_1 + y_2) &=
\begin{pmatrix}
x_1 + x_2 & 0\\
y_2 + y_2 & 0
\end{pmatrix} \\
&=
\begin{pmatrix}
x_1 & 0\\
y_1 & 0
\end{pmatrix}
+
\begin{pmatrix}
x_2 & 0\\
y_2 & 0
\end{pmatrix}
\\
&= f(x_1, y_1) + f(x_2, y_2)
\end{align*}

$$f((x_1, y_1) \otimes (x_2, y_2)) = f(x_1x_2, y_1x_2) =
\begin{pmatrix}
x_1 x_2 & 0\\
y_1 x_2 & 0
\end{pmatrix}
$$
$$f(x_1, y_1)f(x_2y_2) =
\begin{pmatrix}
x_1 & 0\\
y_1 & 0
\end{pmatrix}
\begin{pmatrix}
x_2 & 0\\
y_2 & 0
\end{pmatrix}
=
\begin{pmatrix}
x_1 x_2 & 0\\
y_1 x_2 & 0
\end{pmatrix}
$$
$$K = \{(0, 0)\}$$

## Q6

$$h: P_C \rightarrow P_C$$
$$h(A) = A \cap D$$
$$D \subseteq C$$
\begin{align*}
h(A + B) &= h((A - B) \cup (B - A)) \\
&= [(A - B) \cup (B - A)] \cap D \\
&= [(A - B) \cap D] \cup [(B - A) \cap D] \\
&= [A\cap D - B \cap D] \cup [B \cap D - A \cap D] \\
&= h(A) + h(B) \\
h(AB) &= h(A \cap B) = A \cap B \cap D \\
&= (A \cap D) \cap (B \cap D) \\
&= h(A) h(B)
\end{align*}
$$K = \{ A \in P_C : A \cap D = \varnothing \}$$
Range is every subset of $D$.

## Q7

Rules for ring homomorphisms:
$$f(a + b) = f(a) + f(b) \qquad f(ab) = f(a)f(b)$$
$$f(0) = 0 \qquad f(1_A) = 1_B$$
$$f(n) = f(1 + \cdots + 1) = f(1) + \cdots + f(1) = nf(1)$$
$$mf(1) = 0 \qquad f(1)^2 = f(1)$$

Homomorphisms for $\phi_i : \mathbb{Z}_2 \rightarrow \mathbb{Z}_4$
$$\phi_e =
\begin{pmatrix}
0 & 1\\
0 & 0
\end{pmatrix}$$

The other mappings do not work:

* $1 \rightarrow 1$ then $2 f(1) \neq 0$
* $1 \rightarrow 2$ then $f(1)^2 \neq f(1)$
* $1 \rightarrow 3$ then $f(1)^2 \neq f(1)$

Homomorphisms for $\phi_i : \mathbb{Z}_2 \rightarrow \mathbb{Z}_4$
$$\phi_e =
\begin{pmatrix}
0 & 1 & 2\\
0 & 0 & 0
\end{pmatrix}$$
$$\phi_a =
\begin{pmatrix}
0 & 1 & 2\\
0 & 4 & 2
\end{pmatrix}$$

The other mappings do not work:

* $1 \rightarrow 1$ then $f(1)^2 \neq f(1)$
* $1 \rightarrow 2$ then $f(1)^2 \neq f(1)$
* $1 \rightarrow 3$ then $3f(1) \neq 0$
* $1 \rightarrow 5$ then $3f(1) \neq 0$

# F. Elementary Properties of Homomorphisms

## Q1

*Prove $f(A) = \{ f(x) : x \in A \}$ is a subring of $B$.*

Since $f$ is a homomorphism, ring operations are obeyed in the homomorphism. For negatives we note that $f(0_A) = 0_B = 1_B + (-1_B)$ and every negative is expressible as $(-1_B) \cdot a$ where $a \in B$.

## Q2

*Prove the kernel of $f$ is an ideal of $A$.*

$$K = \{ x \in A: f(x) = 0_B \}$$

From $f$ being a homomorphism, we conclude $K$ is a subring of $A$.

To show it's an ideal, for any $a \in A$ and $x \in K$, then $f(ax) = 0 = f(x)$. So $K$ absorbs the product $ax$.

Thus the kernel of a homomorphism is an ideal of the input ring.

## Q3

*Prove $f(0) = 0$, and for every $a \in A, f(-a) = -f(a)$.*

$$f(0) = f(0 + 0) = f(0) + f(0) \implies f(0) = 0$$
$$f(a + (-a)) = f(a) + f(-a) = f(0) = 0 = f(a) - f(a)$$
$$\implies f(-a) = -f(a)$$

## Q4

*Prove $f$ is injective iff its kernel is equal to $\{ 0 \}$.*

$$f(x) = f(y) \iff f(y - x) = 0 \iff y - x \in K$$

Let $x \in K$

$\implies f(x) = 0$

$\implies f(x) = f(0) \qquad \text{[since $f(0) = 0$]}$

$\implies x = 0 \qquad \text{[since $f$ is injective]}$

It follow $K = \{ 0 \}$

Thus $f$ is injective $\implies K = \{ 0 \}$

Now suppose $K = \{ 0 \}$. Then

$f(x) = f(y)$

$\implies f(x) - f(y) = 0$

$\implies f(x - y) = 0$

$\implies x - y \in K$

$\implies x - y = 0 \qquad \text{[since $K = \{ 0 \}$]}$

$\implies x = y$

Hence $f$ is injective.

Thus $K = \{ 0 \} \implies f$ is injective.

Hence $f$ is injective $\iff K = \{ 0 \}$

## Q5

*If $B$ is an integral domain, then either $f(1) = 1$ or $f(1) = 0$. If $f(1) = 0$ then $f(x) = 0$ for every $x \in A$. If $f(1) = 1$, the image of every invertible element of $A$ is an invertible element of $B$.*

Integral domain has the cancellation property such that $ab = ac \implies b = c$.

$$f(1) = f(1 \cdot 1) = f(1)f(1)$$
$$f(1) = f(1)f(1)$$
$f(1) = 0 \text{ or } 1$$

If $f(1) = 0$ then $\forall a \in A$, $f(a) = f(1 \cdot a) = f(1) f(a) = 0$

If $f(1) = 1$ and $\exists x, y \in A$ such that $xy = 1$

$$f(xy) = f(x)f(y) \text{ where } f(y) = (f(x))^{-1}$$

## Q6

*Any homomorphic image of a commutative ring is a commutative ring. Any homomorphic image of a field is a field.*

Let $a, b \in A$, then $f(a)f(b) = f(b)f(a)$ because $f(ab) = f(ba)$.

If $A$ is a field, then $\forall x \in A$, $\exists x^{-1} \in A$. So by the last exercise, $f(x^{-1}) = (f(x))^{-1}$ and so the inverse of $f(x)$ is a member of $B$.
$$ (f(x))^{-1} \in B$$

## Q7

*If the domain $A$ of the homomorphism $f$ is a field, and if the range of $f$ has more than one element, then $f$ is injective.*

Since $A$ is a field, the kernel of $A$ is either $\{0\}$ or $A$ itself.

But the range of $f$ is more than one element, so the kernel of $A$ cannot be $A$ and must be $\{0\}$.

Since the kernel of $f$ is $\{0\}$, then $f$ is injective.

# G. Examples of Isomorphisms

## Q1

$$a \oplus b = a + b + 1$$
$$a \otimes b = ab + a + b$$

### Addition

\begin{align*}
f(a + b) &= a + b - 1 \\
f(a) \oplus f(b) &= (a - 1) + (b - 1) - 1 \\
&= a + b - 1
\end{align*}

### Multiplication

\begin{align*}
f(ab) &= ab - 1 \\
f(a) \otimes f(b) &= (a - 1)(b - 1) + (a - 1) + (b - 1) \\
&= ab - b - a + 1 + a + b - 1 - 1 \\
&= ab - 1
\end{align*}

## Q2

$$\mathcal{J} = \{
\begin{pmatrix}
a & b\\
-b & a
\end{pmatrix}
: a, b \in \mathbb{R} \}$$
$$f: \mathbb{C} \rightarrow \mathcal{J}$$
$$f(a + bi) = 
\begin{pmatrix}
a & b\\
-b & a
\end{pmatrix}$$
$$a + bi = c + di \implies f(a + bi) = f(c + di)$$

### Addition

\begin{align*}
f((a + bi) + (c + di)) &=
\begin{pmatrix}
a + c & b + d\\
-(b + d) & a + c
\end{pmatrix} \\
f(a + bi) + f(c + di) &=
\begin{pmatrix}
a + c & b + d\\
-(b + d) & a + c
\end{pmatrix} \\
\end{align*}

### Multiplication

\begin{align*}
f((a + bi)(c + di)) &= f((ac - bd) + (ad + bc)i) \\
&=
\begin{pmatrix}
a + c & b + d\\
-(b + d) & a + c
\end{pmatrix} \\
f(a + bi)f(c + di) &=
\begin{pmatrix}
a & b\\
-b & a
\end{pmatrix}
\begin{pmatrix}
c & d\\
-d & c
\end{pmatrix} \\
&=
\begin{pmatrix}
a + c & b + d\\
-(b + d) & a + c
\end{pmatrix} \\
\end{align*}

## Q3

$$A = \{(x, x) : x \in \mathbb{Z}\}$$
$\forall x, y \in \mathbb{Z}, (x, x) \in A, (y, y) \in A, (x + y, x + y) \in A \text{ and } (xy, xy) \in A$

Thus $A$ is a subring of $\mathbb{Z} \times \mathbb{Z}$

The homomorphism $f: \mathbb{Z} \rightarrow A$ by $f(x) = (x, x)$ is isomorphic because it is one to one
$$f(x) = f(y) \implies x = y$$
and onto
$$\forall (x, x) \in A, \exists x \in \mathbb{Z} \text{ such that } f(x) = (x, x)$$

Thus
$$\{(x, x): x \in \mathbb{Z}\} \cong \mathbb{Z}$$

## Q4

Addition and negatives trivially remain inside the set.
$$
\begin{pmatrix}
0 & 0\\
0 & x
\end{pmatrix}
\begin{pmatrix}
0 & 0\\
0 & y
\end{pmatrix}
=
\begin{pmatrix}
0 & 0\\
0 & xy
\end{pmatrix}
$$
Hence the set is a subring.
$$A = \{
\begin{pmatrix}
0 & 0\\
0 & x
\end{pmatrix}
: x \in \mathbb{R}\}$$
Define $f: \mathbb{R} \rightarrow A$ by $f(x) =
\begin{pmatrix}
0 & 0\\
0 & x
\end{pmatrix}$, then $f$ is an homomorphism from $\mathbb{R}$ to $A$.

Hence $A \cong \mathbb{R}$

## Q5

$$f : k \mathbb{Z} \rightarrow l \mathbb{Z}$$
$$f(k) = ln \text{ for some } n \neq 0$$

\begin{align*}
f(k^2) &= l^2 n^2 \\
       &= f(k \cdot k) = f(k + \cdots + k) = k f(k) \\
       &= kln \\
    k &= ln
\end{align*}

But $k \neq l$, so $ln$ does not generate $l \mathbb{Z}$ and $f$ is not an isomorphism.

# H. Further Properties of Ideals

## Q1

*If $J \cap K = \{ 0 \}$, then $jk = 0$ for every $j \in J$ and $k \in K$.*

$J$ and $K$ are ideals, so for every $j \in J$ and $k \in K$, then $jk \in J$ and $jk \in K$, so $jk \in J \cap K$.

## Q2

*For any $a \in A$, $I_a = \{ ax + j + k : x \in A, j \in J, k \in K \}$ is an ideal of $A$.*

$\forall i \in I_a$, and $b \in A$, then $bi = b(ax + j + k) = a(bx) + bj + bk \in I_a$ since $J$ and $K$ are ideals and $bx \in A$.

## Q3

*The radical of $J$ is the set $\rad J = \{ a \in A : a^n \in J \text{ for some } n \in \mathbb{Z} \}$. For any ideal $J$, $\rad J$ is an ideal of $A$.*

$$a^n \in J \qquad b^m \in J$$
$$(a + b)^{n + m} \in J \qquad \text{[see 17m3]}$$

$x \in A$ and $a \in \rad J$ then $(xa)^n = x^n a^n \in J$, so $xa \in \rad J$.

$a, b \in \rad J$, then $(a + b)^{m + n} \in J$ and so $a + b \in \rad J$.

## Q4

*For any $a \in A$, $\{ x \in A : ax = 0 \}$ is an ideal (called the annihilator of $a$).*

*Furthermore, $\{ x \in A : ax = 0 \text{ for every } a \in A \}$ is an ideal (called the annihilating ideal of $A$). If $A$ is a ring with unity, its annihilating ideal is equal to $\{ 0 \}$.*

Let $b \in A$, then $bx \in Ann(a)$ because $ax = 0$ so $b(ax) = bxa = 0$.

Let $x, y \in Ann(a)$ then $a(x + y) = 0$ so $x + y \in Ann(a)$.

$$I = \{ x \in A : ax = 0 \text{ for every } a \in A \}$$

If $A$ is a ring with unity then $a = 1 \implies x = 0$ so $I = \{ 0 \}$.

## Q5

*Show that $\{0\}$ and $A$ are ideals of $A$. (They are trivial ideals; every other ideal of $A$ is a proper ideal.) A proper $J$ of $A$ is called maximal if it is not strictly contained in any strictly larger proper ideal: that is if $J \subseteq K$, where $K$ is an ideal containing some element not in $J$, then necessarily $K = A$.*

*Show the following is an example of a maximal ideal: in $\mathcal{F}(\mathbb{R})$, the ideal $J = \{ f : f(0) = 0 \}$.*

$$g \in K \qquad g(0) \neq 0 \qquad g \notin J$$

$$ h(x) = g(x) - g(0) \in J$$
$$h(x) - g(x) \in K$$

Continuous function with a nonzero value is invertible.

$h(x) - g(x) = -g(0) \in K$ but $g(0) \neq 0$ so $-1/g(0) \in A$.

But since $K$ is an ideal, that is
$$g(0) \cdot 1 / g(0) \in K$$
but this equals $1$, and $1 \in K$ so $K = A$ and is maximal.

# I. Further Properties of Homomorphisms

## Q1

*If $f: A \rightarrow B$ is a homomorphism from $A$ onto $B$ with kernel $K$, and $J$ is an ideal of $A$ such that $K \subseteq J$, then $f(J)$ is an ideal of B$.*

$f$ is onto $\exists x: f(x) = y$ so it's an ideal. Closed under addition and negatives and absorbs products.

See also [here](https://math.stackexchange.com/questions/2200335/is-the-homomorphic-image-of-an-ideal-an-ideal)

## Q2

*If $f : A \rightarrow B$ is a homomorphism from $A$ onto $B$, and $B$ is a field, then the kernel of $f$ is a maximal ideal.*

The kernel $K$ is a subset of the ideal for $A$. As shown above $f(J)$ is an ideal of $B$, which by D6 can only be $\{0\}$ or $B$ itself. Since the homomorphism is onto, then $f(A)$ maps to $B$, but $A$ is a trivial ideal of $A$. Thus $K$, the kernel of $f$ is the proper ideal for $A$ which maps to $\{0\}$ in $B$.

## Q3

*There are no nontrivial homomorphisms from $\mathbb{Z}$ to $\mathbb{Z}$.*

$$f(1) = f(1 \cdot 1) = f(1) \cdot f(1)$$
$$f(1) = 1 \text{ or } f(1) = 0$$
$$f(n) = f(1 + \cdots + 1) = f(1) + \cdots + f(1) = nf(1)$$

So $f(n) = n$ or $f(n) = 0$

See also [here](https://math.stackexchange.com/questions/1625916/showing-there-are-no-nontrivial-ring-homomorphisms-from-mathbbz-to-mathbbz) and [here](https://math.stackexchange.com/questions/1517973/ring-homomorphism-from-mathbb-z-to-mathbb-z-is-always-identity-or-0)

## Q4

*If $n$ is a multiple of $m$, then $\mathbb{Z}_m$ is a homomorphic image of $\mathbb{Z}_n$.*

$f: \mathbb{Z}_n \rightarrow \mathbb{Z}_m$$ by $f(a) = a (\mod m)$ obeys the homomorphic properties.

See also [here](https://math.stackexchange.com/questions/2517417/given-that-m-divides-n-show-that-z-m-is-a-homomorphic-image-of-z-n)

## Q5

*If $n$ is odd, there is an injective homomorphism from $\mathbb{Z}_2$ into $\mathbb{Z}_{2n}$.*

$$f(x) = nx$$

Above homomorphism is injective since $f(0) = 0$ and $f(1) = n$.

# J. A Ring of Endomorphisms

## Q1

$$\pi_a(x) = ax$$
$$\pi_a(x + y) = a(x + y) = ax + ay = \pi_a(x) + \pi_a(y)$$

## Q2

$$\pi_a(x) = \pi_a(y) \implies x = y$$

$a$ is not a divisor of zero $\implies \forall x \in A, ax \neq 0$, thus ring $A$ has cancellation property
$$\pi_a(x) = \pi_a(y) = ax = ay \implies x = y$$

## Q3

If $a$ is invertible then $\forall y \in A$, $y = a(a^{-1}y)$ so $x = a^{-1}y$, $f(x) = y$, thus $\pi_a$ is surjective.

## Q4

$$\mathcal{A} = \{ \pi_a : a \in A \}$$
$$[\pi_a + \pi_b](x) = \pi_a(x) + \pi_b(x)$$
$$\pi_a\pi_b = \pi_a \cdot \pi_b$$

1. Addition is abelian
2. Multiplication is associative: $(\pi_a \cdot \pi_b \cdot \pi_c)(x) = (abc)x = a(bcx) = \pi_a((\pi_b \cdot \pi_c)(x))$
3. Distributive over addition

## Q5

$$\phi: A \rightarrow \mathcal{A} \text{ given by } \phi(a) = \pi_a$$
As shown above this is homomorphic.

## Q6

$$\phi(a) = \phi(b) \implies \pi_a = \pi_b$$
$$\pi_a(1) = \pi_b(1) \implies a = b$$

$\forall \pi_a \in \mathcal{A}, \exists a \in A : \pi_a = \phi(a)$ by definition.

If $a$ has no divisors of zero, then to show injective property, note that
$$ax = bx \implies a = b$$
$$\pi_a = pi_b \implies \pi_a(x) = ax = \pi_b(x) = bx \implies a = b$$

From the cancellation property since it has no divisors of zero.

